InternalNondet.v
@@ -3,16 +3,16 @@ Require Import TraceModel.
 Require Import Properties.
 Require Import CommonST.
 Require Import Robustdef.
-Require Import Criteria. 
+Require Import Criteria.
 Require Import ClassicalExtras.
 
 (** This file proves the collapses that happens in presence of
     a non-deterministic choice operator in the source language *)
 
 
-(* 
+(*
 
-   RrHP ------ 
+   RrHP ------
                \
     |          RrSCP----
                /          \
@@ -23,7 +23,7 @@ Require Import ClassicalExtras.
    RHP--- /            /             |
          /            /              |
     |   /            /               |
-       /            /                | 
+       /            /                |
    RSCP  --------- /                 |
                   /-                 |
     |            /                   /
@@ -32,17 +32,17 @@ Require Import ClassicalExtras.
                                   /
                                  /
    / \                          /
-                               / 
- RDP  RSP (<-> RFrSP) --------- 
+                               /
+ RDP  RSP (<-> RFrSP) ---------
 
 *)
 
-Variable nd  : ctx src -> ctx src -> ctx src.
+Variable nd  : ctx src i -> ctx src i -> ctx src i.
 
 Infix "⊕" := nd (at level 50).
 
 
-Axiom nd_beh1 : forall C1 C2 P, beh (C1 [P]) ⊆ beh ((C1 ⊕ C2) [P]).  
+Axiom nd_beh1 : forall C1 C2 P, beh (C1 [P]) ⊆ beh ((C1 ⊕ C2) [P]).
 
 Axiom nd_beh2 : forall C1 C2 P, beh (C2 [P]) ⊆ beh ((C1 ⊕ C2) [P]).
 
@@ -50,25 +50,25 @@ Axiom nd_beh2 : forall C1 C2 P, beh (C2 [P]) ⊆ beh ((C1 ⊕ C2) [P]).
 (** *RSP -> R2rSP *)
 (* and with a similar argument RSP -> R r_fin SP *)
 
-Lemma RSC' : RSC <-> forall P Ct m, psem (Ct[P↓]) m -> exists Cs, psem (Cs[P]) m.
+Lemma RSC' : RSC <-> forall (P : par src i) Ct m, psem (Ct[P↓]) m -> exists Cs, psem (Cs[P]) m.
 Proof.
   split.
   + intros rsc P Ct m [t [Hpref Hsem]].
     destruct (rsc P Ct t Hsem m Hpref) as [Cs [t' [Hsem' Hpref']]].
     exists Cs. now exists t'.
-                + intros rsc' P Ct t Hsem m Hpref.                
+                + intros rsc' P Ct t Hsem m Hpref.
                   destruct (rsc' P Ct m) as  [Cs [t' [Hpref' Hsem']]].
                   now exists t.
                         now exists Cs, t'.
 Qed.
 
-Lemma RSP_R2rSP : RSC -> R2rSC. 
+Lemma RSP_R2rSP : RSC -> R2rSC.
 Proof.
-  rewrite RSC'. 
+  rewrite RSC'.
   intros rsc Ct P1 P2 m1 m2 H1 H2.
   destruct (rsc P1 Ct m1) as [Cs1 [t1 [Hpref1 Hs1]]]; auto.
   destruct (rsc P2 Ct m2) as [Cs2 [t2 [Hpref2 Hs2]]]; auto.
-  exists (Cs1 ⊕ Cs2). unfold psem. split; [exists t1 | exists t2]; split; auto.   
+  exists (Cs1 ⊕ Cs2). unfold psem. split; [exists t1 | exists t2]; split; auto.
   now apply nd_beh1. now apply nd_beh2.
 Qed.
 
@@ -76,14 +76,14 @@ Qed.
 (** *RTP -> R2rTP *)
 (* and with a similar argument RTP -> R r_fin TP *)
 
-Lemma RTP_R2rTP : RTP -> R2rTP. 
+Lemma RTP_R2rTP : RTP -> R2rTP.
 Proof.
   rewrite <- RTC_RTP, <- R2rTC_R2rTP.
   intros Hrc Ct P1 P2 t1 t2 H1 H2.
   destruct (Hrc P1 Ct t1) as [Cs1 Hs1]. specialize (Hs1 H1).
   destruct (Hrc P2 Ct t2) as [Cs2 Hs2]. specialize (Hs2 H2).
   exists (Cs1 ⊕ Cs2). split; [apply nd_beh1 | apply nd_beh2]; auto.
-Qed.   
+Qed.
 
 (** *RTP -> R2rTP *)
 (* and with a similar argument RTP -> R r_fin TP *)
@@ -106,12 +106,11 @@ Qed.
 (*   rewrite two_scC.  *)
 (*   intros rc P1 P2 Ct. *)
 (* Abort. *)
-(*we should apply rc for every t ∈ beh (ct[P1 ↓]) to get Cs_1 and 
-                     for every t ∈ beh (ct[P2 ↓]) to get Cs_2, then 
-  apply ⊕ and get the desired context. 
+(*we should apply rc for every t ∈ beh (ct[P1 ↓]) to get Cs_1 and
+                     for every t ∈ beh (ct[P2 ↓]) to get Cs_2, then
+  apply ⊕ and get the desired context.
   When one of these two sets is infinite ⊕ should be applied infinitely many times
 
-  Assuming finitary non determinism the implication can be proved.  
+  Assuming finitary non determinism the implication can be proved.
 
  *)
-
