R2rXP_RTEP.v
@@ -9,16 +9,16 @@ Require Import List.
 
 Require Import XPrefix.
 Require Import Criteria.
-Require Import TechnicalLemmas. 
+Require Import TechnicalLemmas.
 
 (** *our assumptions *)
 (**********************************************************)
-Hypothesis input_totality_tgt : input_totality tgt.
-Hypothesis determinacy_src    : determinacy src.
-Hypothesis tgt_sem           : semantics_safety_like tgt.
+Hypothesis input_totality_tgt : @input_totality tgt.
+Hypothesis determinacy_src    : @determinacy src.
+Hypothesis tgt_sem            : @semantics_safety_like tgt.
 (**********************************************************)
 
-  
+
 Lemma three_continuations_tbd :
   forall l t, xprefix (xtbd l) t ->
          ( (exists e, t = tstop l e) \/
@@ -28,15 +28,15 @@ Proof.
   intros l [] Hpref.
   + simpl in Hpref. apply list_proper_or_equal in Hpref. destruct Hpref.
     ++ subst. left. now exists e.
-    ++ right. right. firstorder.  
+    ++ right. right. firstorder.
   + simpl in Hpref. apply list_proper_or_equal in Hpref. destruct Hpref.
     ++ subst. right. now left.
-    ++ right. right. firstorder. 
+    ++ right. right. firstorder.
   + generalize dependent s. induction l.
-    ++ right. right. destruct s. now exists e. 
+    ++ right. right. destruct s. now exists e.
     ++ intros [] Hpref. inversion Hpref. simpl.
        destruct (IHl s) as [ [ef FALSE] | [ FALSE | [e0 HH] ]]; try now inversion FALSE; auto.
-       now simpl. right. right. exists e0; firstorder.  
+       now simpl. right. right. exists e0; firstorder.
 Qed.
 
 
@@ -52,7 +52,7 @@ Definition myXr (x1 x2: xpref) : Prop :=
 
 
 Lemma myXr_symmetric : forall x1 x2, myXr x1 x2 -> myXr x2 x1.
- Proof. firstorder. Qed. 
+ Proof. firstorder. Qed.
 
 Lemma auXiliary_tstop :
   forall x2 l1 e1 t2, xprefix x2 t2 ->
@@ -61,32 +61,32 @@ Proof.
   intros x2 l1 e1 t2 xprefix2 [Heq | [ll [i1 [i2 [I1 [I2 [Idiff [l_prefix1 l_prefix2]]]]]]]].
   + rewrite <- Heq in *. destruct (xsame_ext (xstop l1 e1) x2 (tstop l1 e1)); simpl; auto;
                           [now left |  right; now left].
-  + destruct x2, t2; simpl in xprefix2; simpl in l_prefix1, l_prefix2; try now auto.   
-    ++ inversion xprefix2; subst.  
+  + destruct x2, t2; simpl in xprefix2; simpl in l_prefix1, l_prefix2; try now auto.
+    ++ inversion xprefix2; subst.
        right. right. now exists ll, i1, i2.
     ++ destruct (list_list_same_ext l (snoc ll i2) l0); auto.
-       * destruct (list_proper_or_equal _ _ H) as [HH | [a HH]].        
+       * destruct (list_proper_or_equal _ _ H) as [HH | [a HH]].
          ** subst. right. right. now exists ll, i1, i2.
          ** apply list_pref_snoc_pref in HH.
             right. left. simpl. apply (list_list_prefix_trans l (snoc ll i1) l1);auto.
-            apply (list_list_prefix_trans l ll _); auto. now apply snoc_longer. 
-       * right. right. now exists ll, i1, i2.  
+            apply (list_list_prefix_trans l ll _); auto. now apply snoc_longer.
+       * right. right. now exists ll, i1, i2.
     ++ destruct (list_list_same_ext l (snoc ll i2) l0); auto.
-       * destruct (list_proper_or_equal _ _ H) as [HH | [a HH]].        
+       * destruct (list_proper_or_equal _ _ H) as [HH | [a HH]].
          ** subst. right. right. now exists ll, i1, i2.
          ** apply list_pref_snoc_pref in HH.
             right. left. simpl. apply (list_list_prefix_trans l (snoc ll i1) l1);auto.
-            apply (list_list_prefix_trans l ll _); auto. now apply snoc_longer. 
+            apply (list_list_prefix_trans l ll _); auto. now apply snoc_longer.
        * right. right. now exists ll, i1, i2.
     ++ destruct (list_stream_same_ext l (snoc ll i2) s); auto.
-       * destruct (list_proper_or_equal _ _ H) as [HH | [a HH]].        
+       * destruct (list_proper_or_equal _ _ H) as [HH | [a HH]].
          ** subst. right. right. now exists ll, i1, i2.
          ** apply list_pref_snoc_pref in HH.
             right. left. simpl. apply (list_list_prefix_trans l (snoc ll i1) l1);auto.
-            apply (list_list_prefix_trans l ll _); auto. now apply snoc_longer. 
-       * right. right. now exists ll, i1, i2.  
-    ++ subst. right. right. now exists ll, i1, i2. 
-Qed. 
+            apply (list_list_prefix_trans l ll _); auto. now apply snoc_longer.
+       * right. right. now exists ll, i1, i2.
+    ++ subst. right. right. now exists ll, i1, i2.
+Qed.
 
 Lemma auXiliary_tsilent :
   forall x2 l1 t2, xprefix x2 t2 ->
@@ -95,32 +95,32 @@ Proof.
   intros x2 l1 t2 xprefix2 [Heq | [ll [i1 [i2 [I1 [I2 [Idiff [l_prefix1 l_prefix2]]]]]]]].
   + rewrite <- Heq in *. destruct (xsame_ext (xsilent l1) x2 (tsilent l1)); simpl; auto;
                           [now left |  right; now left].
-   + destruct x2, t2; simpl in xprefix2; simpl in l_prefix1, l_prefix2; try now auto.   
-    ++ inversion xprefix2; subst.  
+   + destruct x2, t2; simpl in xprefix2; simpl in l_prefix1, l_prefix2; try now auto.
+    ++ inversion xprefix2; subst.
        right. right. now exists ll, i1, i2.
     ++ destruct (list_list_same_ext l (snoc ll i2) l0); auto.
-       * destruct (list_proper_or_equal _ _ H) as [HH | [a HH]].        
+       * destruct (list_proper_or_equal _ _ H) as [HH | [a HH]].
          ** subst. right. right. now exists ll, i1, i2.
          ** apply list_pref_snoc_pref in HH.
             right. left. simpl. apply (list_list_prefix_trans l (snoc ll i1) l1);auto.
-            apply (list_list_prefix_trans l ll _); auto. now apply snoc_longer. 
-       * right. right. now exists ll, i1, i2.  
+            apply (list_list_prefix_trans l ll _); auto. now apply snoc_longer.
+       * right. right. now exists ll, i1, i2.
     ++ destruct (list_list_same_ext l (snoc ll i2) l0); auto.
-       * destruct (list_proper_or_equal _ _ H) as [HH | [a HH]].        
+       * destruct (list_proper_or_equal _ _ H) as [HH | [a HH]].
          ** subst. right. right. now exists ll, i1, i2.
          ** apply list_pref_snoc_pref in HH.
             right. left. simpl. apply (list_list_prefix_trans l (snoc ll i1) l1);auto.
-            apply (list_list_prefix_trans l ll _); auto. now apply snoc_longer. 
+            apply (list_list_prefix_trans l ll _); auto. now apply snoc_longer.
        * right. right. now exists ll, i1, i2.
     ++ destruct (list_stream_same_ext l (snoc ll i2) s); auto.
-       * destruct (list_proper_or_equal _ _ H) as [HH | [a HH]].        
+       * destruct (list_proper_or_equal _ _ H) as [HH | [a HH]].
          ** subst. right. right. now exists ll, i1, i2.
          ** apply list_pref_snoc_pref in HH.
             right. left. simpl. apply (list_list_prefix_trans l (snoc ll i1) l1);auto.
-            apply (list_list_prefix_trans l ll _); auto. now apply snoc_longer. 
-       * right. right. now exists ll, i1, i2.  
+            apply (list_list_prefix_trans l ll _); auto. now apply snoc_longer.
+       * right. right. now exists ll, i1, i2.
     ++ subst. right. right. now exists ll, i1, i2.
-Qed. 
+Qed.
 
 
 Lemma auXiliary_xtbd:
@@ -128,134 +128,134 @@ Lemma auXiliary_xtbd:
                   traces_match t1 t2 -> myXr (xtbd l1) (xtbd l2).
 Proof.
   intros l1 l2 t1 t2 xpref1 xpref2 [Heq | [ll [i1 [i2 [I1 [I2 [Idiff [l_prefix1 l_prefix2]]]]]]]].
-  + subst. destruct (xsame_ext (xtbd l1) (xtbd l2) t2); auto; [now left | right; now left]. 
+  + subst. destruct (xsame_ext (xtbd l1) (xtbd l2) t2); auto; [now left | right; now left].
   + assert (H1: xprefix (xtbd (snoc ll i1)) t1).
     { destruct t1; simpl in *; now auto. }
     assert (H2 : xprefix (xtbd (snoc ll i2)) t2).
     { destruct t2; simpl in *; now auto. }
-    destruct (xsame_ext (xtbd l1) (xtbd (snoc ll i1)) t1) as [l1_shorter | l1_longer]; auto. 
+    destruct (xsame_ext (xtbd l1) (xtbd (snoc ll i1)) t1) as [l1_shorter | l1_longer]; auto.
     ++ destruct (xsame_ext (xtbd l2) (xtbd (snoc ll i2)) t2) as [l2_shorter | l2_longer]; auto.
        destruct (list_proper_or_equal _ _ l1_shorter) as [l1_ll | [a1 l1_ll]]; subst.
-       * destruct (list_proper_or_equal _ _ l2_shorter) as [l2_ll | [a2 l2_ll]]; subst. 
-          ** right. right. now exists ll, i1, i2. 
+       * destruct (list_proper_or_equal _ _ l2_shorter) as [l2_ll | [a2 l2_ll]]; subst.
+          ** right. right. now exists ll, i1, i2.
           ** apply list_pref_snoc_pref in l2_ll. right. left. simpl.
-             apply (list_list_prefix_trans l2 ll _); auto. now apply snoc_longer.  
+             apply (list_list_prefix_trans l2 ll _); auto. now apply snoc_longer.
        * apply list_pref_snoc_pref in l1_ll.
-         destruct (list_proper_or_equal _ _ l2_shorter) as [l2_ll | [a2 l2_ll]]; subst. 
-         **  left. simpl. apply (list_list_prefix_trans l1 ll _ ); auto. now apply snoc_longer.  
+         destruct (list_proper_or_equal _ _ l2_shorter) as [l2_ll | [a2 l2_ll]]; subst.
+         **  left. simpl. apply (list_list_prefix_trans l1 ll _ ); auto. now apply snoc_longer.
          ** apply list_pref_snoc_pref in l2_ll. destruct (list_list_same_ext l1 l2 ll); auto;
-                                                  [now left | right; now left].  
-       * destruct (list_proper_or_equal  _ _ l1_shorter); auto; subst. 
-         ** right. right. now exists ll, i1, i2.  
+                                                  [now left | right; now left].
+       * destruct (list_proper_or_equal  _ _ l1_shorter); auto; subst.
+         ** right. right. now exists ll, i1, i2.
          ** destruct H as [a H]. apply list_pref_snoc_pref in H. left.
             simpl. apply (list_list_prefix_trans l1 ll l2); auto.
             simpl in l2_longer. apply (list_list_prefix_trans ll (snoc ll i2) l2); auto.
-            now apply snoc_longer.  
+            now apply snoc_longer.
     ++ destruct (xsame_ext (xtbd l2) (xtbd (snoc ll i2)) t2) as [l2_shorter | l2_longer]; auto.
-       * destruct (list_proper_or_equal _ _ l2_shorter) as [l2_ll | [a2 l2_ll]]; subst. 
-          ** right. right. now exists ll, i1, i2. 
+       * destruct (list_proper_or_equal _ _ l2_shorter) as [l2_ll | [a2 l2_ll]]; subst.
+          ** right. right. now exists ll, i1, i2.
           ** apply list_pref_snoc_pref in l2_ll. right. left. simpl.
              apply (list_list_prefix_trans l2 ll _); auto.
              apply (list_list_prefix_trans ll (snoc ll i1) _); auto. now apply snoc_longer.
         * right. right. now exists ll, i1, i2.
-Qed.   
-    
+Qed.
+
 
 Lemma auXiliary_lemma (t1 t2 : trace) :
   traces_match t1 t2 ->
   forall x1 x2,  xprefix x1 t1 -> xprefix x2 t2 -> myXr x1 x2.
 Proof.
-  intros [Heq | [ll [i1 [i2 [I1 [I2 [Idiff [l_prefix1 l_prefix2]]]]]]]] x1 x2 xprefix1 xprefix2. 
-  - subst. unfold myXr. destruct (xsame_ext x1 x2 t2) as [go_left | go_right_left]; auto. 
+  intros [Heq | [ll [i1 [i2 [I1 [I2 [Idiff [l_prefix1 l_prefix2]]]]]]]] x1 x2 xprefix1 xprefix2.
+  - subst. unfold myXr. destruct (xsame_ext x1 x2 t2) as [go_left | go_right_left]; auto.
   - destruct x1, x2.
     ++ destruct t1, t2; inversion xprefix1; inversion xprefix2; subst.
        right. right. now exists ll, i1, i2.
-    ++ destruct t1; inversion xprefix1; subst.  
+    ++ destruct t1; inversion xprefix1; subst.
        apply (auXiliary_tstop (xtbd l0) l1 e0 t2); auto.
-       right. now exists ll, i1, i2. 
+       right. now exists ll, i1, i2.
     ++ destruct t1, t2; inversion xprefix1; inversion xprefix2; subst.
        simpl in *. right. right. now exists ll, i1, i2.
-    ++ destruct t2; inversion xprefix2; subst. apply myXr_symmetric. 
+    ++ destruct t2; inversion xprefix2; subst. apply myXr_symmetric.
        apply (auXiliary_tstop (xtbd l) l1 e0 t1); auto.
-       right. exists ll, i2, i1. repeat (split; try now auto). 
-    ++ apply (auXiliary_xtbd l l0 t1 t2); auto. right. now exists ll, i1, i2.  
-    ++ destruct t2; inversion xprefix2; subst. apply myXr_symmetric.  
+       right. exists ll, i2, i1. repeat (split; try now auto).
+    ++ apply (auXiliary_xtbd l l0 t1 t2); auto. right. now exists ll, i1, i2.
+    ++ destruct t2; inversion xprefix2; subst. apply myXr_symmetric.
        apply (auXiliary_tsilent (xtbd l) l1 t1); auto.
-       right. exists ll, i2, i1. repeat (split; try now auto).  
+       right. exists ll, i2, i1. repeat (split; try now auto).
     ++ destruct t1, t2; inversion xprefix1; inversion xprefix2; subst.
        simpl in *. right. right. now exists ll, i1, i2.
-    ++ destruct t1; inversion xprefix1; subst.   
+    ++ destruct t1; inversion xprefix1; subst.
        apply (auXiliary_tsilent (xtbd l0) l1 t2); auto.
        right. now exists ll, i1, i2.
     ++ destruct t1, t2; inversion xprefix1; inversion xprefix2; subst.
-       simpl in *. right. right. now exists ll, i1, i2.   
-Qed. 
-  
-Lemma teq_premises_myXr_holds : forall P1 P2,
+       simpl in *. right. right. now exists ll, i1, i2.
+Qed.
+
+Lemma teq_premises_myXr_holds : forall (P1 P2 : par src i),
     (forall Cs t, sem src (Cs [P1]) t <-> sem src (Cs [P2]) t) ->
     (forall Cs x1 x2, xsem (Cs [P1]) x1 -> xsem (Cs [P2]) x2 ->
                  myXr x1 x2).
 Proof.
   intros P1 P2 H Cs x1 x2 [t1 [xpref1 sem1]] [t2 [xpref2 sem2]].
     rewrite (H Cs t1) in sem1.
-   specialize (determinacy_src (Cs[P2]) t1 t2 sem1 sem2). 
+   specialize (determinacy_src (Cs[P2]) t1 t2 sem1 sem2).
    intros Hmatch. now apply (auXiliary_lemma t1 t2).
 Qed.
-    
+
 
 Lemma  longest_in_xsem :
   forall W t, ~ sem tgt W t ->
     exists x, xprefix x t /\ xsem W x /\
      (forall x', xprefix x' t -> xsem W x' -> xpr x' x).
 Proof.
-  intros W [] HsemWt.  
+  intros W [] HsemWt.
   + destruct (list_longest_in_psem W l) as [ll [Hpref [Hpsem Hmax]]].
-    exists (xtbd ll). repeat (split; try now auto). 
+    exists (xtbd ll). repeat (split; try now auto).
     intros [] Hx Hsemx.
     ++ inversion Hx; subst. destruct Hsemx as [tx [Hprefxtx Hsemx]].
-       destruct tx; inversion Hprefxtx; subst. contradiction.  
-    ++ simpl in *. apply Hmax; auto. 
-    ++ inversion Hx. 
+       destruct tx; inversion Hprefxtx; subst. contradiction.
+    ++ simpl in *. apply Hmax; auto.
+    ++ inversion Hx.
   + destruct (list_longest_in_psem W l) as [ll [Hpref [Hpsem Hmax]]].
-    exists (xtbd ll). repeat (split; try now auto). 
+    exists (xtbd ll). repeat (split; try now auto).
     intros [] Hx Hsemx.
-    ++ inversion Hx; subst.   
-    ++ simpl in *. apply Hmax; auto. 
+    ++ inversion Hx; subst.
+    ++ simpl in *. apply Hmax; auto.
     ++ inversion Hx; subst. simpl in *.
        destruct Hsemx as [tx [Hprefxtx Hsemx]].
        destruct tx; inversion Hprefxtx; subst. contradiction.
-  + destruct (tgt_sem (tstream s) W) as [l [ebad [Hseml [Hprefl Hnsem_longer]]]]; auto. 
+  + destruct (tgt_sem (tstream s) W) as [l [ebad [Hseml [Hprefl Hnsem_longer]]]]; auto.
     exists (xtbd l). simpl in *. repeat (split; try now auto).
     ++ apply (list_stream_prefix_trans l (snoc l ebad) s); auto.
        now apply snoc_longer.
-    ++ intros [] Hpref_x HxsemW; try now inversion Hpref_x.   
+    ++ intros [] Hpref_x HxsemW; try now inversion Hpref_x.
        simpl in *. destruct (list_stream_same_ext l0 (snoc l ebad) s); auto.
        * apply list_proper_or_equal in H. destruct H as [H | [a H]].
-         ** subst. exfalso. apply Hnsem_longer. destruct HxsemW as [tx [H1 H2]]. 
-                 now exists tx. 
+         ** subst. exfalso. apply Hnsem_longer. destruct HxsemW as [tx [H1 H2]].
+                 now exists tx.
          ** now apply list_pref_snoc_pref in H.
        * exfalso. apply Hnsem_longer. destruct HxsemW as [tx [H1 H2]].
              exists tx. split; try now auto.
-             destruct tx; simpl in *; try now apply (list_list_prefix_trans (snoc l ebad) l0 l1). 
+             destruct tx; simpl in *; try now apply (list_list_prefix_trans (snoc l ebad) l0 l1).
              now apply (list_stream_prefix_trans (snoc l ebad) l0 s0).
 Qed.
 
 
 Lemma input_tot_consequence (W : prg tgt): forall l i1 i2,
-    is_input i1 -> is_input i2 -> 
+    is_input i1 -> is_input i2 ->
     xsem W (xtbd (snoc l i1)) -> xsem W (xtbd (snoc l i2)).
 Proof.
   intros l i1 i2 Hi1 Hi2 [t [xpref_x_t Hsemt]].
   assert (psem W (ftbd  (snoc l i1))).
   { simpl in *. now exists t. }
   now apply (input_totality_tgt W l i1 i2) in H.
-Qed.  
+Qed.
 
-Lemma t_being_tstop_leads_to_contra (W1 W2 : prg tgt) t l2 e2 
+Lemma t_being_tstop_leads_to_contra (W1 W2 : prg tgt) t l2 e2
                                     (sem1 : sem tgt W1 t) (sem2 : sem tgt W2 (tstop l2 e2))
                                     (nsem12: ~ sem tgt W2 t)
                                     (xpref_x_t : xprefix (xtbd l2) t)
-  : 
+  :
     (forall x1 x2, xsem W1 x1 -> xsem W2 x2 -> myXr x1 x2) -> False.
 Proof.
  intros twoX. destruct t.
@@ -263,81 +263,81 @@ Proof.
      as [xpr1 | [xpr2 | [xx [i1 [i2 [Hi1 [Hi2 [Hdiff [Hxpr1 Hxpr2]]]]]]]]].
    now exists (tstop l e). now exists (tstop l2 e2).
    + inversion xpr1; subst. contradiction.
-   + inversion xpr2; subst. contradiction.                                
+   + inversion xpr2; subst. contradiction.
    + simpl in Hxpr1, Hxpr2.
-     apply (list_list_prefix_trans (snoc xx i2) l2 l Hxpr2) in xpref_x_t.   
+     apply (list_list_prefix_trans (snoc xx i2) l2 l Hxpr2) in xpref_x_t.
      destruct (list_list_same_ext (snoc xx i1) (snoc xx i2) l) as [F | F]; auto;
        apply Hdiff; apply (list_snoc_diff xx _ _ ) in F; congruence.
  - simpl in xpref_x_t.  destruct (twoX (xsilent l) (xstop l2 e2))
      as [xpr1 | [xpr2 | [xx [i1 [i2 [Hi1 [Hi2 [Hdiff [Hxpr1 Hxpr2]]]]]]]]].
-    now exists (tsilent l). try now exists (tstop l2 e2).  
-    + now inversion xpr1.                              
+    now exists (tsilent l). try now exists (tstop l2 e2).
+    + now inversion xpr1.
     + now inversion xpr2.
     + simpl in Hxpr1, Hxpr2.
-     apply (list_list_prefix_trans (snoc xx i2) l2 l Hxpr2) in xpref_x_t.   
+     apply (list_list_prefix_trans (snoc xx i2) l2 l Hxpr2) in xpref_x_t.
      destruct (list_list_same_ext (snoc xx i1) (snoc xx i2) l) as [F | F]; auto;
        apply Hdiff; apply (list_snoc_diff xx _ _ ) in F; congruence.
  - simpl in xpref_x_t.
-   destruct (tgt_sem (tstream s) W2 nsem12) as [l [ebad [Hpsem [Hpref Hnpsem]]]]; auto. 
+   destruct (tgt_sem (tstream s) W2 nsem12) as [l [ebad [Hpsem [Hpref Hnpsem]]]]; auto.
    simpl in Hpref.
    destruct (twoX (xtbd (snoc l ebad)) (xstop l2 e2))
-     as [xpr1 | [xpr2 | [xx [i1 [i2 [Hi1 [Hi2 [Hdiff [Hxpr1 Hxpr2]]]]]]]]]; auto.  
+     as [xpr1 | [xpr2 | [xx [i1 [i2 [Hi1 [Hi2 [Hdiff [Hxpr1 Hxpr2]]]]]]]]]; auto.
    now exists (tstream s). now exists (tstop l2 e2).
    + simpl in xpr1. apply Hnpsem. now exists (tstop l2 e2).
    + simpl in *.
-     apply (list_stream_prefix_trans _ _ s) in Hxpr1; auto.  
-     apply (list_stream_prefix_trans _ _ s) in Hxpr2; auto.  
-     destruct (list_stream_same_ext (snoc xx i1) (snoc xx i2) s) as [F | F]; auto;                              apply Hdiff; apply (list_snoc_diff xx _ _) in F; congruence.         
-Qed. 
+     apply (list_stream_prefix_trans _ _ s) in Hxpr1; auto.
+     apply (list_stream_prefix_trans _ _ s) in Hxpr2; auto.
+     destruct (list_stream_same_ext (snoc xx i1) (snoc xx i2) s) as [F | F]; auto;                              apply Hdiff; apply (list_snoc_diff xx _ _) in F; congruence.
+Qed.
 
-Lemma t_being_tsilent_leads_to_contra (W1 W2 : prg tgt) t l2  
+Lemma t_being_tsilent_leads_to_contra (W1 W2 : prg tgt) t l2
                                       (sem1 : sem tgt W1 t) (sem2 : sem tgt W2 (tsilent l2))
                                       (nsem12: ~ sem tgt W2 t)
                                       (xpref_x_t : xprefix (xtbd l2) t)
-  : 
+  :
     (forall x1 x2, xsem W1 x1 -> xsem W2 x2 -> myXr x1 x2) -> False.
 Proof.
  intros twoX. destruct t.
  - simpl in *. destruct (twoX (xstop l e) (xsilent l2))
      as [xpr1 | [xpr2 | [xx [i1 [i2 [Hi1 [Hi2 [Hdiff [Hxpr1 Hxpr2]]]]]]]]].
    now exists (tstop l e). now exists (tsilent l2).
-   + now inversion xpr1. 
-   + now inversion xpr2.                                
+   + now inversion xpr1.
+   + now inversion xpr2.
    + simpl in Hxpr1, Hxpr2.
-     apply (list_list_prefix_trans (snoc xx i2) l2 l Hxpr2) in xpref_x_t.   
+     apply (list_list_prefix_trans (snoc xx i2) l2 l Hxpr2) in xpref_x_t.
      destruct (list_list_same_ext (snoc xx i1) (snoc xx i2) l) as [F | F]; auto;
        apply Hdiff; apply (list_snoc_diff xx _ _ ) in F; congruence.
  - simpl in xpref_x_t.  destruct (twoX (xsilent l) (xsilent l2))
      as [xpr1 | [xpr2 | [xx [i1 [i2 [Hi1 [Hi2 [Hdiff [Hxpr1 Hxpr2]]]]]]]]].
-    now exists (tsilent l). try now exists (tsilent l2).  
-    + simpl in xpr1. now subst.                              
-    + simpl in xpr2. now subst. 
+    now exists (tsilent l). try now exists (tsilent l2).
+    + simpl in xpr1. now subst.
+    + simpl in xpr2. now subst.
     + simpl in Hxpr1, Hxpr2.
-     apply (list_list_prefix_trans (snoc xx i2) l2 l Hxpr2) in xpref_x_t.   
+     apply (list_list_prefix_trans (snoc xx i2) l2 l Hxpr2) in xpref_x_t.
      destruct (list_list_same_ext (snoc xx i1) (snoc xx i2) l) as [F | F]; auto;
        apply Hdiff; apply (list_snoc_diff xx _ _ ) in F; congruence.
  - simpl in xpref_x_t.
-   destruct (tgt_sem (tstream s) W2 nsem12) as [l [ebad [Hpsem [Hpref Hnpsem]]]]; auto. 
+   destruct (tgt_sem (tstream s) W2 nsem12) as [l [ebad [Hpsem [Hpref Hnpsem]]]]; auto.
    simpl in Hpref.
    destruct (twoX (xtbd (snoc l ebad)) (xsilent l2))
-     as [xpr1 | [xpr2 | [xx [i1 [i2 [Hi1 [Hi2 [Hdiff [Hxpr1 Hxpr2]]]]]]]]]; auto.  
+     as [xpr1 | [xpr2 | [xx [i1 [i2 [Hi1 [Hi2 [Hdiff [Hxpr1 Hxpr2]]]]]]]]]; auto.
    now exists (tstream s). now exists (tsilent l2).
    + simpl in xpr1. apply Hnpsem. now exists (tsilent l2).
    + simpl in *.
-     apply (list_stream_prefix_trans _ _ s) in Hxpr1; auto.  
-     apply (list_stream_prefix_trans _ _ s) in Hxpr2; auto.  
-     destruct (list_stream_same_ext (snoc xx i1) (snoc xx i2) s) as [F | F]; auto;                              apply Hdiff; apply (list_snoc_diff xx _ _) in F; congruence.         
-Qed. 
- 
+     apply (list_stream_prefix_trans _ _ s) in Hxpr1; auto.
+     apply (list_stream_prefix_trans _ _ s) in Hxpr2; auto.
+     destruct (list_stream_same_ext (snoc xx i1) (snoc xx i2) s) as [F | F]; auto;                              apply Hdiff; apply (list_snoc_diff xx _ _) in F; congruence.
+Qed.
+
 
 Lemma violates_xmax  (W1 W2 : prg tgt) t t2 l a aa
                      (sem1 : sem tgt W1 t) (sem2 : sem tgt W2 t2)
                      (nsem12: ~ sem tgt W2 t)
                      (xpref_x_t : xprefix (xtbd (snoc l aa)) t)
                      (x_t2 : xprefix (xtbd (snoc l a)) t2)
-                       
+
   :
-    (forall x' : xpref, xprefix x' t -> xsem W2 x' -> xpr x' (xtbd l)) -> 
+    (forall x' : xpref, xprefix x' t -> xsem W2 x' -> xpr x' (xtbd l)) ->
     (forall x1 x2, xsem W1 x1 -> xsem W2 x2 ->  myXr x1 x2) -> False.
 Proof.
   intros xmax twoX.
@@ -347,31 +347,31 @@ Proof.
   destruct twoX as [xpr1 | [xpr2 | matching]].
   + simpl in xpr1. apply list_snoc_diff in xpr1. subst.
     specialize (xmax (xtbd (snoc l a)) xpref_x_t xsem2).
-    simpl in xmax. now apply snoc_strictly_longer in xmax. 
+    simpl in xmax. now apply snoc_strictly_longer in xmax.
   + simpl in xpr2. apply list_snoc_diff in xpr2. subst.
     specialize (xmax (xtbd (snoc l aa)) xpref_x_t xsem2).
-    simpl in xmax. now apply snoc_strictly_longer in xmax. 
+    simpl in xmax. now apply snoc_strictly_longer in xmax.
   + destruct matching as [xx [i1 [i2 [Hi1 [Hi2 [Hdiff_is [Hxpr1 Hxpr2 ]]]]]]].
-    simpl in Hxpr1, Hxpr2.  
-    apply (list_snoc_pointwise xx l i1 i2 aa a) in Hxpr2; auto.  
+    simpl in Hxpr1, Hxpr2.
+    apply (list_snoc_pointwise xx l i1 i2 aa a) in Hxpr2; auto.
     destruct Hxpr2 as [H1 H2]. subst.
-    apply (input_tot_consequence W2 l a aa) in xsem2; auto. 
+    apply (input_tot_consequence W2 l a aa) in xsem2; auto.
     specialize (xmax (xtbd (snoc l aa)) xpref_x_t xsem2).
-    simpl in xmax. now apply snoc_strictly_longer in xmax. 
-Qed. 
-    
+    simpl in xmax. now apply snoc_strictly_longer in xmax.
+Qed.
 
-Lemma tinp_premises_myXr_holds : forall P1 P2,
+
+Lemma tinp_premises_myXr_holds : forall (P1 P2 : par src i),
     (forall Cs t, sem src (Cs [P1]) t -> sem src (Cs [P2]) t) ->
     (forall Cs x1 x2, xsem (Cs [P1]) x1 -> xsem (Cs [P2]) x2 ->
                  myXr x1 x2).
 Proof.
   intros P1 P2 H Cs x1 x2 [t1 [xpref1 sem1]] [t2 [xpref2 sem2]].
   apply (H Cs t1) in sem1.
-   specialize (determinacy_src (Cs[P2]) t1 t2 sem1 sem2). 
+   specialize (determinacy_src (Cs[P2]) t1 t2 sem1 sem2).
    intros Hmatch. now apply (auXiliary_lemma t1 t2).
 Qed.
-     
+
 Theorem R2rXP_RTIP : R2rXP -> RTIP.
 Proof.
   rewrite <- R2rXC_R2rXP, R2rXC_R2rXC'. unfold R2rXC', RTIP, beh.
@@ -384,33 +384,33 @@ Proof.
     destruct x.
     ++ (* it can only be t2 '=' xstop p e = t *)
        destruct t, t2; auto.
-       inversion xpref_x_t; inversion x_t2; subst; congruence.  
+       inversion xpref_x_t; inversion x_t2; subst; congruence.
     ++ destruct (three_continuations_tbd l t2 x_t2) as [t2stop | [t2silent | t2longer]].
-       +++ destruct t2stop as [e2 Ht2]. rewrite Ht2 in *. 
+       +++ destruct t2stop as [e2 Ht2]. rewrite Ht2 in *.
            now apply (t_being_tstop_leads_to_contra (Ct [P1↓]) (Ct [P2↓]) t l e2).
-       +++ rewrite t2silent in *. 
-           now apply (t_being_tsilent_leads_to_contra  (Ct [P1↓]) (Ct [P2↓]) t l).         
+       +++ rewrite t2silent in *.
+           now apply (t_being_tsilent_leads_to_contra  (Ct [P1↓]) (Ct [P2↓]) t l).
        +++ destruct t2longer as [a t2longer].
            destruct (three_continuations_tbd l t xpref_x_t) as [ttstop | [ttsilent | ttlonger]].
-           - destruct ttstop as [e ttstop]. subst. 
+           - destruct ttstop as [e ttstop]. subst.
              destruct (twoX (xstop l e) (xtbd (snoc l a))) as [xpr1 | [xpr2 | matching]]; auto.
-             now exists (tstop l e). now exists t2. 
-             -- simpl in xpr2. now apply snoc_strictly_longer in xpr2. 
-             -- destruct matching as [xx [i1 [i2 [Hi1 [Hi2 [Hdiff [Hxpr1 Hxpr2 ]]]]]]].
-                simpl in Hxpr1, Hxpr2. 
-                apply (snocs_aux_lemma xx l i2 i1 a); congruence.       
-           - subst. 
-             destruct (twoX (xsilent l) (xtbd (snoc l a))) as [xpr1 | [xpr2 | matching]]; auto.
-             now exists (tsilent l). now exists t2. 
+             now exists (tstop l e). now exists t2.
              -- simpl in xpr2. now apply snoc_strictly_longer in xpr2.
              -- destruct matching as [xx [i1 [i2 [Hi1 [Hi2 [Hdiff [Hxpr1 Hxpr2 ]]]]]]].
                 simpl in Hxpr1, Hxpr2.
-                apply (snocs_aux_lemma xx l i2 i1 a); congruence. 
+                apply (snocs_aux_lemma xx l i2 i1 a); congruence.
+           - subst.
+             destruct (twoX (xsilent l) (xtbd (snoc l a))) as [xpr1 | [xpr2 | matching]]; auto.
+             now exists (tsilent l). now exists t2.
+             -- simpl in xpr2. now apply snoc_strictly_longer in xpr2.
+             -- destruct matching as [xx [i1 [i2 [Hi1 [Hi2 [Hdiff [Hxpr1 Hxpr2 ]]]]]]].
+                simpl in Hxpr1, Hxpr2.
+                apply (snocs_aux_lemma xx l i2 i1 a); congruence.
            - destruct ttlonger as [aa ttlonger].
-             now apply (violates_xmax (Ct [P1↓]) (Ct [P2↓]) t t2 l a aa).              
+             now apply (violates_xmax (Ct [P1↓]) (Ct [P2↓]) t t2 l a aa).
    ++ (*  it can only be t2 '=' xsilent p e = t *)
-      destruct t, t2; auto. 
-      inversion xpref_x_t; inversion x_t2; subst; congruence. 
+      destruct t, t2; auto.
+      inversion xpref_x_t; inversion x_t2; subst; congruence.
 Qed.
 
 
